Commented blake2.fst compiler output to point out problems

spec-compilers/fstar/speclib.fst
@@ -19,25 +19,32 @@ let uint32_v x = uint_v #U32 x
 unfold let range i = i
 
 val split_blocks: #a:Type -> s:seq a -> bs:size_nat{bs > 0} -> (bl:seq (lseq a bs){length bl == length s / bs} * l:seq a{length l == length s % bs})
-let split_blocks #a (s:seq a) (bs:size_nat{bs > 0}) = 
+let split_blocks #a (s:seq a) (bs:size_nat{bs > 0}) =
   let (bl,l) = split_blocks (to_lseq s) bs in
   (to_seq bl, to_seq l)
 
-val concat_blocks: #a:Type -> #len:size_nat -> #bs:size_nat{bs > 0} -> 
+val concat_blocks: #a:Type -> #len:size_nat -> #bs:size_nat{bs > 0} ->
   bl:seq (lseq a bs){length bl == len / bs} -> l:seq a{length l == len % bs} ->
   r:seq a{length r == len}
 let concat_blocks #_ #len #bs bl l =
   to_seq (concat_blocks #_ #len #bs (to_lseq bl) (to_lseq l))
 
-let rec exp (x:nat) (y:nat) = 
+let rec exp (x:nat) (y:nat) =
     if y = 0 then 1
     else x `op_Multiply` (exp x (y-1))
-let ( **. ) x y = 
+let ( **. ) x y =
   if x = 2 then pow2 y
   else exp x y
 type pfelem_t (p:nat) = x:nat{x < p}
 let pfelem (p:pos) (x:nat): pfelem_t p = x % p
 let pfelem_to_int x = x
-let pfadd #p (x:pfelem_t p) (y:pfelem_t p) : pfelem_t p = pfelem p (x + y) 
+let pfadd #p (x:pfelem_t p) (y:pfelem_t p) : pfelem_t p = pfelem p (x + y)
 let ( -. ) x y = x - y
 
+val uints_from_bytes_le: #a:inttype -> s:seq uint8_t{length s % (numbytes a) = 0} -> r:seq (uint_t a){length r = (length s) / (numbytes a)}
+let uints_from_bytes_le #a s =
+  to_seq (uints_from_bytes_le #a #((length s) / (numbytes a)) (to_lseq s))
+
+val uints_to_bytes_le: #a:inttype -> s:seq (uint_t a){FStar.Mul.op_Star (length s) (numbytes a) <= max_size_t} -> r:seq uint8_t{length r = FStar.Mul.op_Star (length s) (numbytes a)}
+let uints_to_bytes_le #a s =
+  to_seq (uints_to_bytes_le #a #(length s) (to_lseq s))
